src/Common/SumType.v
@@ -1,0 +1,108 @@
+Require Import
+        Coq.Vectors.Vector
+        Coq.Vectors.VectorDef.
+
+Require Import
+        Fiat.Common.BoundedLookup.
+
+Import Coq.Vectors.VectorDef.VectorNotations.
+Local Open Scope vector_scope.
+Local Open Scope string_scope.
+
+Fixpoint SumType {n} (v : Vector.t Type n) {struct v} : Type :=
+  match v with
+  | Vector.nil => (False : Type)
+  | Vector.cons T _ Vector.nil => T
+  | Vector.cons T _ v' => T + (SumType v')
+  end%type.
+
+Arguments SumType : simpl never.
+
+Fixpoint inj_SumType {n}
+         (v : Vector.t Type n)
+         (tag : Fin.t n)
+         (el : Vector.nth v tag)
+         {struct v} : SumType v.
+  refine (match v in Vector.t _ n return
+                forall
+                  (tag : Fin.t n)
+                  (el : Vector.nth v tag),
+                  SumType v
+          with
+          | Vector.nil => fun tag el => Fin.case0 _ tag
+          | Vector.cons T n' v' => fun tag el => _
+          end tag el).
+
+  generalize v' (inj_SumType n' v') el0; clear; pattern n', tag0; apply Fin.caseS; simpl; intros.
+  - destruct v'; simpl.
+    + exact el0.
+    + exact (inl el0).
+  - destruct v'; simpl.
+    + exact (Fin.case0 _ p).
+    + exact (inr (X p el0)).
+Defined.
+
+Fixpoint SumType_index {n}
+         (v : Vector.t Type n)
+         (el : SumType v)
+         {struct v} : Fin.t n.
+  refine (match v in Vector.t _ n return
+                SumType v -> Fin.t n
+          with
+          | Vector.nil => fun el => match el with end
+          | Vector.cons T _ v' => fun el => _
+          end el).
+  generalize (SumType_index _ v'); clear SumType_index; intros.
+  destruct v'; simpl.
+  - exact Fin.F1.
+  - destruct el0.
+    + exact Fin.F1.
+    + exact (Fin.FS (X s)).
+Defined.
+
+Fixpoint SumType_proj {n}
+         (v : Vector.t Type n)
+         (el : SumType v)
+         {struct v} : v[@SumType_index v el].
+  refine (match v in Vector.t _ n return
+                forall el : SumType v, v[@SumType_index v el]
+          with
+          | Vector.nil => fun el => match el with end
+          | Vector.cons T _ v' => fun el => _
+          end el).
+  generalize (SumType_proj _ v'); clear SumType_proj; intros.
+  destruct v'; simpl.
+  - exact el0.
+  - destruct el0.
+    + exact t.
+    + exact (X s).
+Defined.
+
+Lemma inj_SumType_proj_inverse {n}
+  : forall (v : Vector.t Type n)
+           (el : SumType v),
+    inj_SumType v _ (SumType_proj v el) = el.
+Proof.
+  induction v; simpl; intros.
+  - destruct el.
+  - destruct v.
+    + simpl; reflexivity.
+    + destruct el; simpl; eauto.
+      f_equal; apply IHv.
+Qed.
+
+Lemma index_SumType_inj_inverse {n}
+  : forall  (tag : Fin.t n)
+            (v : Vector.t Type n)
+            (el : Vector.nth v tag),
+    SumType_index v (inj_SumType v tag el) = tag.
+Proof.
+  induction tag.
+  - intro; pattern n, v; eapply Vector.caseS; simpl.
+    clear; intros; destruct t; eauto.
+  - intro; revert tag IHtag; pattern n, v; eapply Vector.caseS; simpl; intros.
+    destruct t.
+    + inversion tag.
+    + f_equal.
+      eapply IHtag.
+Qed.
